---
title: "Variance of a Binomial"
author: "Justin Kleiber"
date: "`r Sys.Date()`"
output: 
  html_document: 
    toc: yes
    toc_float: yes
---

```{r setup, include=FALSE}
knitr::opts_chunk$set(echo = TRUE, message = FALSE)
```

# Introduction

We have learnt that the MGF for a binomial random variable is:

$$M_X(t) = (q+pe^t)^n $$

Where $X\sim Bin(n,p)$

# Tasks

Using the moment generating function above prove that 

$$\sigma^2 = npq$$

by answering the tasks below. 
Use $\LaTeX$ to construct the proof.

## Task 1

Start with 

$$
\begin{eqnarray}
E(X) &=& \left . \frac{d M_X(t)}{dt}\right |_{t=0}\\
&=& npe^t(q + pe^t)^{n-1} |_{t=0}\\
&=& np(q + p)^{n-1}\\
&=& np
\end{eqnarray}
$$


## Task 2

Now find $E(X^2)$

$$
\begin{eqnarray}
E(X^2) &=& \frac{d^2M_X(t)}{dt^2} |_{t=0}\\
&=& n(n-1)pe^t(q+pe^t)^{n-2}pe^t + pe^tn(q+pe^t)^{n-1} |_{t=0}\\
&=& n(n-1)p(q+p)^{n-2}p + np(q+p)^{n-1} |_{t=0}\\
&=& n(n-1)p^2 + np\\
&=& n^2p^2 - np^2 + np\\
&=& n(np^2 + p - p^2)\\
&=& n(np^2 + p(1-p))\\
&=& n(np^2 + pq)\\
&=& (np)^2 + npq
\end{eqnarray}
$$

## Task 3

Find $\sigma^2$ Using the formula $\sigma^2 = E(X^2)-\mu^2$

$$
\begin{eqnarray}
\mu &=& E(X) = np\\
\mu^2 &=& (np)^2\\
E(X^2) &=& (np)^2 + npq\\
\sigma^2 &=& E(X^2)-\mu^2\\
\sigma^2 &=& (np)^2 + npq - (np)^2\\
\sigma^2 &=& npq
\end{eqnarray}
$$
